feature(wasm) per-module extraction and add wasm_ast to compiler
Signed-off-by: Jerome Simeon <jeromesimeon@me.com>

compiler/lib/check_util.ml
@@ -15,7 +15,7 @@
 (* Result checking *)
 
 open Format
-open Core.EnhancedCompiler
+open EnhancedCompiler.EnhancedCompiler
 open Config_util
 
 (* Check result *)
